library/init/meta/smt/interactive.lean
@@ -228,18 +228,18 @@ slift (tactic.interactive.induction p rec_name ids revert)
 open tactic
 
 /-- Simplify the target type of the main goal. -/
-meta def simp (hs : parse opt_qexpr_list) (attr_names : parse with_ident_list) (ids : parse without_ident_list) (cfg : simp_config := {}) : smt_tactic unit :=
-tactic.interactive.simp hs attr_names ids (loc.ns []) cfg
+meta def simp (no_dflt : parse only_flag) (hs : parse opt_qexpr_list) (attr_names : parse with_ident_list) (ids : parse without_ident_list) (cfg : simp_config := {}) : smt_tactic unit :=
+tactic.interactive.simp no_dflt hs attr_names ids (loc.ns []) cfg
 
 /-- Simplify the target type of the main goal using simplification lemmas and the current set of hypotheses. -/
-meta def simp_using_hs (hs : parse opt_qexpr_list) (attr_names : parse with_ident_list) (ids : parse without_ident_list) (cfg : simp_config := {}) : smt_tactic unit :=
-tactic.interactive.simp_using_hs hs attr_names ids cfg
+meta def simp_using_hs (no_dflt : parse only_flag) (hs : parse opt_qexpr_list) (attr_names : parse with_ident_list) (ids : parse without_ident_list) (cfg : simp_config := {}) : smt_tactic unit :=
+tactic.interactive.simp_using_hs no_dflt hs attr_names ids cfg
 
-meta def simph (hs : parse opt_qexpr_list) (attr_names : parse with_ident_list) (ids : parse without_ident_list) (cfg : simp_config := {}) : smt_tactic unit :=
-simp_using_hs hs attr_names ids cfg
+meta def simph (no_dflt : parse only_flag) (hs : parse opt_qexpr_list) (attr_names : parse with_ident_list) (ids : parse without_ident_list) (cfg : simp_config := {}) : smt_tactic unit :=
+simp_using_hs no_dflt hs attr_names ids cfg
 
-meta def dsimp (es : parse opt_qexpr_list) (attr_names : parse with_ident_list) (ids : parse without_ident_list) : smt_tactic unit :=
-tactic.interactive.dsimp es attr_names ids (loc.ns [])
+meta def dsimp (no_dflt : parse only_flag) (es : parse opt_qexpr_list) (attr_names : parse with_ident_list) (ids : parse without_ident_list) : smt_tactic unit :=
+tactic.interactive.dsimp no_dflt es attr_names ids (loc.ns [])
 
 meta def rsimp : smt_tactic unit :=
 do ccs ← to_cc_state, _root_.rsimp.rsimplify_goal ccs
